pagedb.s/i: split validDispatcherContext from wellformedDispatcherContext

verified/pagedb.s.dfy
@@ -66,7 +66,7 @@ predicate physPageIsSecure(physPage: int)
 
 datatype PageDbEntryTyped
     = Addrspace(l1ptnr: PageNr, refcount: nat, state: AddrspaceState)
-    | Dispatcher(entrypoint:int, entered:bool, ctxt:DispatcherContext)
+    | Dispatcher(entrypoint:word, entered:bool, ctxt:DispatcherContext)
     | L1PTable(l1pt: seq<Maybe<PageNr>>)
     | L2PTable(l2pt: seq<L2PTE>)
     | DataPage
@@ -102,7 +102,7 @@ predicate wellFormedPageDbEntryTyped(e: PageDbEntryTyped)
 {
     (e.L1PTable? ==> |e.l1pt| == NR_L1PTES())
     && (e.L2PTable? ==> |e.l2pt| == NR_L2PTES())
-    && (e.Dispatcher? ==> validDispatcherContext(e.ctxt))
+    && (e.Dispatcher? ==> wellformedDispatcherContext(e.ctxt))
 }
 
 predicate {:opaque} validPageDb(d: PageDb)
@@ -118,12 +118,17 @@ lemma validPageDbImpliesWellFormed(d:PageDb)
     ensures wellFormedPageDb(d)
     { reveal_validPageDb(); }
 
-predicate validDispatcherContext(dc:DispatcherContext)
+predicate wellformedDispatcherContext(dc:DispatcherContext)
 {
     R0 in dc.regs && R1 in dc.regs && R2 in dc.regs && R3 in dc.regs
     && R4  in dc.regs && R5  in dc.regs && R6  in dc.regs && R7  in dc.regs
     && R8  in dc.regs && R9  in dc.regs && R10 in dc.regs && R11 in dc.regs
     && R12 in dc.regs && LR(User) in dc.regs && SP(User) in dc.regs
+}
+
+predicate validDispatcherContext(dc:DispatcherContext)
+{
+    wellformedDispatcherContext(dc)
     && decode_mode'(psr_mask_mode(dc.cpsr)) == Just(User)
 }
 
